VST-introduction/sum.v
@@ -74,22 +74,12 @@ Definition ___compcert_va_composite : ident := $"__compcert_va_composite".
 Definition ___compcert_va_float64 : ident := $"__compcert_va_float64".
 Definition ___compcert_va_int32 : ident := $"__compcert_va_int32".
 Definition ___compcert_va_int64 : ident := $"__compcert_va_int64".
-Definition ___stringlit_1 : ident := $"__stringlit_1".
 Definition _a : ident := $"a".
 Definition _b : ident := $"b".
 Definition _main : ident := $"main".
-Definition _printf : ident := $"printf".
 Definition _result : ident := $"result".
 Definition _sum_2_2 : ident := $"sum_2_2".
 Definition _t'1 : ident := 128%positive.
-
-Definition v___stringlit_1 := {|
-  gvar_info := (tarray tschar 4);
-  gvar_init := (Init_int8 (Int.repr 37) :: Init_int8 (Int.repr 100) ::
-                Init_int8 (Int.repr 10) :: Init_int8 (Int.repr 0) :: nil);
-  gvar_readonly := true;
-  gvar_volatile := false
-|}.
 
 Definition f_sum_2_2 := {|
   fn_return := tint;
@@ -119,13 +109,7 @@ Definition f_main := {|
     (Ssequence
       (Scall (Some _t'1) (Evar _sum_2_2 (Tfunction nil tint cc_default)) nil)
       (Sset _result (Etempvar _t'1 tint)))
-    (Ssequence
-      (Scall None
-        (Evar _printf (Tfunction ((tptr tschar) :: nil) tint
-                        {|cc_vararg:=(Some 1); cc_unproto:=false; cc_structret:=false|}))
-        ((Evar ___stringlit_1 (tarray tschar 4)) ::
-         (Etempvar _result tint) :: nil))
-      (Sreturn (Some (Econst_int (Int.repr 0) tint)))))
+    (Sreturn (Some (Etempvar _result tint))))
   (Sreturn (Some (Econst_int (Int.repr 0) tint))))
 |}.
 
@@ -212,7 +196,7 @@ Definition global_definitions : list (ident * globdef fundef type) :=
    Gfun(External (EF_runtime "__compcert_i64_umulh"
                    (mksignature (AST.Xlong :: AST.Xlong :: nil) AST.Xlong
                      cc_default)) (tulong :: tulong :: nil) tulong
-     cc_default)) :: (___stringlit_1, Gvar v___stringlit_1) ::
+     cc_default)) ::
  (___builtin_bswap64,
    Gfun(External (EF_builtin "__builtin_bswap64"
                    (mksignature (AST.Xlong :: nil) AST.Xlong cc_default))
@@ -383,36 +367,30 @@ Definition global_definitions : list (ident * globdef fundef type) :=
                      {|cc_vararg:=(Some 1); cc_unproto:=false; cc_structret:=false|}))
      (tint :: nil) tvoid
      {|cc_vararg:=(Some 1); cc_unproto:=false; cc_structret:=false|})) ::
- (_printf,
-   Gfun(External (EF_external "printf"
-                   (mksignature (AST.Xptr :: nil) AST.Xint
-                     {|cc_vararg:=(Some 1); cc_unproto:=false; cc_structret:=false|}))
-     ((tptr tschar) :: nil) tint
-     {|cc_vararg:=(Some 1); cc_unproto:=false; cc_structret:=false|})) ::
  (_sum_2_2, Gfun(Internal f_sum_2_2)) :: (_main, Gfun(Internal f_main)) ::
  nil).
 
 Definition public_idents : list ident :=
-(_main :: _sum_2_2 :: _printf :: ___builtin_debug ::
- ___builtin_write32_reversed :: ___builtin_write16_reversed ::
- ___builtin_read32_reversed :: ___builtin_read16_reversed ::
- ___builtin_fnmsub :: ___builtin_fnmadd :: ___builtin_fmsub ::
- ___builtin_fmadd :: ___builtin_fmin :: ___builtin_fmax ::
- ___builtin_expect :: ___builtin_unreachable :: ___builtin_va_end ::
- ___builtin_va_copy :: ___builtin_va_arg :: ___builtin_va_start ::
- ___builtin_membar :: ___builtin_annot_intval :: ___builtin_annot ::
- ___builtin_sel :: ___builtin_memcpy_aligned :: ___builtin_sqrt ::
- ___builtin_fsqrt :: ___builtin_fabsf :: ___builtin_fabs ::
- ___builtin_ctzll :: ___builtin_ctzl :: ___builtin_ctz :: ___builtin_clzll ::
- ___builtin_clzl :: ___builtin_clz :: ___builtin_bswap16 ::
- ___builtin_bswap32 :: ___builtin_bswap :: ___builtin_bswap64 ::
- ___compcert_i64_umulh :: ___compcert_i64_smulh :: ___compcert_i64_sar ::
- ___compcert_i64_shr :: ___compcert_i64_shl :: ___compcert_i64_umod ::
- ___compcert_i64_smod :: ___compcert_i64_udiv :: ___compcert_i64_sdiv ::
- ___compcert_i64_utof :: ___compcert_i64_stof :: ___compcert_i64_utod ::
- ___compcert_i64_stod :: ___compcert_i64_dtou :: ___compcert_i64_dtos ::
- ___compcert_va_composite :: ___compcert_va_float64 ::
- ___compcert_va_int64 :: ___compcert_va_int32 :: nil).
+(_main :: _sum_2_2 :: ___builtin_debug :: ___builtin_write32_reversed ::
+ ___builtin_write16_reversed :: ___builtin_read32_reversed ::
+ ___builtin_read16_reversed :: ___builtin_fnmsub :: ___builtin_fnmadd ::
+ ___builtin_fmsub :: ___builtin_fmadd :: ___builtin_fmin ::
+ ___builtin_fmax :: ___builtin_expect :: ___builtin_unreachable ::
+ ___builtin_va_end :: ___builtin_va_copy :: ___builtin_va_arg ::
+ ___builtin_va_start :: ___builtin_membar :: ___builtin_annot_intval ::
+ ___builtin_annot :: ___builtin_sel :: ___builtin_memcpy_aligned ::
+ ___builtin_sqrt :: ___builtin_fsqrt :: ___builtin_fabsf ::
+ ___builtin_fabs :: ___builtin_ctzll :: ___builtin_ctzl :: ___builtin_ctz ::
+ ___builtin_clzll :: ___builtin_clzl :: ___builtin_clz ::
+ ___builtin_bswap16 :: ___builtin_bswap32 :: ___builtin_bswap ::
+ ___builtin_bswap64 :: ___compcert_i64_umulh :: ___compcert_i64_smulh ::
+ ___compcert_i64_sar :: ___compcert_i64_shr :: ___compcert_i64_shl ::
+ ___compcert_i64_umod :: ___compcert_i64_smod :: ___compcert_i64_udiv ::
+ ___compcert_i64_sdiv :: ___compcert_i64_utof :: ___compcert_i64_stof ::
+ ___compcert_i64_utod :: ___compcert_i64_stod :: ___compcert_i64_dtou ::
+ ___compcert_i64_dtos :: ___compcert_va_composite ::
+ ___compcert_va_float64 :: ___compcert_va_int64 :: ___compcert_va_int32 ::
+ nil).
 
 Definition prog : Clight.program := 
   mkprogram composites global_definitions public_idents _main Logic.I.
